\begin{thm}\label{thm:id-adm}
	$\LDL \vdash A \Rightarrow A$.
\end{thm}
\begin{proof}
	By induction on the structure of $A$. If $A$ is an atom, $\bot$ or $\top$, we would have $A \Rightarrow A$ using the axioms of $\LDL$, $Lw$ and $Rw$. If $A = B \circ C$, where $\circ \in \{\wedge, \vee, \supset\}$, the claim is clear from the induction hypothesis for $B$ and $C$. We will explain the proof in details for $A = B \rightarrow C$ and $A = \nabla B$.

If $A = B \rightarrow C$, then we have $B \rightarrow C \Rightarrow B \rightarrow C$ by the following proof-tree. The subtrees denoted by IH are obtained from the induction hypothesis.
\begin{prooftree}
  \AXC{IH} \noLine
  \UIC{$B \Rightarrow B$} \RightLabel{$Lw$}
  \UIC{$\nabla (B \rightarrow C), B \Rightarrow B$}
  \AXC{IH} \noLine
  \UIC{$C \Rightarrow C$} \RightLabel{$Lw$}
  \UIC{$\nabla (B \rightarrow C), C \Rightarrow C$}
  \RightLabel{$L \rightarrow ^n$}
  \BIC{$\nabla (B \rightarrow C), B \Rightarrow C$}
  \RightLabel{$R \rightarrow$}
  \UIC{$B \rightarrow C \Rightarrow B \rightarrow C$}
\end{prooftree}

If $A = \nabla B$, then we can prove $\nabla B \Rightarrow \nabla B$ by applying $N$ on $B \Rightarrow B$, which is proved using induction hypothesis.

\end{proof}